ArrayPtr: support converting from reference

pulse/lib/pulse/lib/Pulse.Lib.ArrayPtr.fst
@@ -20,6 +20,7 @@ module Pulse.Lib.ArrayPtr
 noeq
 type base_t ([@@@strictly_positive] a: Type0) =
 | Null
+| Ref of R.ref a
 | Array of A.array a
 
 let base_length
@@ -28,6 +29,7 @@ let base_length
 : GTot nat
 = match b with
   | Null -> 0
+  | Ref _ -> 1
   | Array a -> A.length a
 
 noeq
@@ -43,9 +45,13 @@ let null #t = { base = Null; offset = 0sz }
 
 let g_is_null p = Null? p.base
 
+let v_is_empty (#t: Type) (s: ptr t) (v: Seq.seq t) : Tot slprop =
+  pure (offset s <= 1 /\ Seq.length v == 0)
+
 let pts_to s #p v =
   match s.base with
   | Array a -> A.pts_to_range a (SZ.v s.offset) (SZ.v s.offset + Seq.length v) #p v
+  | Ref a -> if offset s = 0 && Seq.length v = 1 then R.pts_to a #p (Seq.index v 0) else v_is_empty s v
   | Null -> pure False
 
 ghost fn pts_to_not_null
@@ -63,6 +69,35 @@ ensures
     rewrite emp as (pts_to s #p v)
   } else {
     ()
+  }
+}
+
+ghost fn pts_to_length
+  (#t:Type)
+  (s:ptr t)
+  (#p:perm)
+  (#v : Seq.seq t)
+requires
+  (pts_to s #p v)
+ensures
+  (pts_to s #p v ** pure (offset s + Seq.length v <= base_length (base s)))
+{
+  pts_to_not_null s;
+  if (Array? s.base) {
+    let Array a = s.base;
+    rewrite pts_to s #p v
+      as A.pts_to_range a (SZ.v s.offset) (SZ.v s.offset + Seq.length v) #p v;
+    A.pts_to_range_prop _;
+    rewrite A.pts_to_range a (SZ.v s.offset) (SZ.v s.offset + Seq.length v) #p v
+      as pts_to s #p v;
+  } else if (s.offset = 0sz && Seq.length v = 1) {
+    ()
+  } else {
+    let Ref a = s.base;
+    rewrite (pts_to s #p v) as (v_is_empty s v);
+    unfold (v_is_empty s v);
+    fold (v_is_empty s v);
+    rewrite (v_is_empty s v) as (pts_to s #p v)
   }
 }
 
@@ -116,6 +151,34 @@ fn to_array (#t: Type) (s: ptr t) (a: array t) (#p: perm) (#v: Seq.seq t)
     A.pts_to_range_elim a _ _;
 }
 
+let is_from_ref s a =
+    pure (s.base == Ref a)
+
+fn from_ref (#t: Type) (a: R.ref t) (#p: perm) (#v: Ghost.erased (t))
+    requires R.pts_to a #p v
+    returns s: ptr t
+    ensures pts_to s #p (Seq.create 1 (Ghost.reveal v)) ** is_from_ref s a
+{
+    let res = {
+        base = Ref a;
+        offset = 0sz;
+    };
+    fold (is_from_ref res a);
+    rewrite (R.pts_to a #p v)
+        as (pts_to res #p (Seq.create 1 (Ghost.reveal v)));
+    res
+}
+
+ghost
+fn to_ref (#t: Type) : to_ref_t t
+= (s: ptr t) (a: ref t) (#p: perm) (#v: Seq.seq t)
+{
+    pts_to_length s;
+    unfold is_from_ref s a;
+    rewrite (pts_to s #p v)
+      as (R.pts_to a #p (Seq.index v 0))
+}
+
 fn op_Array_Access
         (#t: Type)
         (a: ptr t)
@@ -132,6 +195,7 @@ fn op_Array_Access
               res == Seq.index s (SZ.v i))
 {
     pts_to_not_null a;
+  if (Array? a.base) {
     let Array ar = a.base;    
     rewrite (pts_to a #p s)
       as (A.pts_to_range ar (SZ.v a.offset) (SZ.v a.offset + Seq.length s) #p s); 
@@ -140,6 +204,14 @@ fn op_Array_Access
     rewrite (A.pts_to_range ar (SZ.v a.offset) (SZ.v a.offset + Seq.length s) #p s)
       as (pts_to a #p s);
     res
+  } else {
+    pts_to_length a;
+    let Ref r = a.base;
+    rewrite (pts_to a #p s) as (R.pts_to r #p (Seq.index s 0));
+    let res = !r;
+    rewrite (R.pts_to r #p (Seq.index s 0)) as (pts_to a #p s);
+    res
+  }
 }
 
 fn op_Array_Assignment
@@ -157,6 +229,7 @@ fn op_Array_Assignment
             )
 {
     pts_to_not_null a;
+  if (Array? a.base) {
     let Array ar = a.base;
     rewrite (pts_to a s)
       as (A.pts_to_range ar (SZ.v a.offset) (SZ.v a.offset + Seq.length s) s);
@@ -167,6 +240,13 @@ fn op_Array_Assignment
     as
       pts_to a (Seq.upd s (SZ.v i) v);
     ();
+  } else {
+    pts_to_length a;
+    let Ref r = a.base;
+    rewrite (pts_to a s) as (R.pts_to r (Seq.index s 0));
+    r := v;
+    rewrite (R.pts_to r v) as (pts_to a (Seq.upd s (SZ.v i) v));
+  }
 }
 
 ghost
@@ -179,6 +259,7 @@ fn share
   ensures pts_to arr #(p /. 2.0R) s ** pts_to arr #(p /. 2.0R) s
 {
     pts_to_not_null arr;
+  if (Array? arr.base) {
     let Array a = arr.base;
     rewrite (pts_to arr #p s)
       as (A.pts_to_range a (SZ.v arr.offset) (SZ.v arr.offset + Seq.length s) #p s);
@@ -187,6 +268,29 @@ fn share
       as (pts_to arr #(p /. 2.0R) s);
     rewrite (A.pts_to_range a (SZ.v arr.offset) (SZ.v arr.offset + Seq.length s) #(p /. 2.0R) s)
       as (pts_to arr #(p /. 2.0R) s);
+  } else {
+    let test = (offset arr = 0 && Seq.length (Ghost.reveal s) = 1);
+    if (test) {
+      let Ref a = arr.base;
+      rewrite (pts_to arr #p s)
+        as (R.pts_to a #p (Seq.index s 0));
+      R.share a;
+      rewrite (R.pts_to a #(p /. 2.0R) (Seq.index s 0))
+        as (pts_to arr #(p /. 2.0R) s);
+      rewrite (R.pts_to a #(p /. 2.0R) (Seq.index s 0))
+        as (pts_to arr #(p /. 2.0R) s);
+    } else {
+      rewrite (pts_to arr #p s)
+        as (v_is_empty arr s);
+      unfold (v_is_empty arr s);
+      fold (v_is_empty arr s);
+      rewrite (v_is_empty arr s)
+        as (pts_to arr #(p /. 2.0R) s);
+      fold (v_is_empty arr s);
+      rewrite (v_is_empty arr s)
+        as (pts_to arr #(p /. 2.0R) s);
+    }
+  }
 }
 
 ghost
@@ -199,6 +303,7 @@ fn gather
   ensures pts_to arr #(p0 +. p1) s0 ** pure (s0 == s1)
 {
     pts_to_not_null arr #p0;
+  if (Array? arr.base) {
     let Array a = arr.base;
     rewrite (pts_to arr #p0 s0)
       as (A.pts_to_range a (SZ.v arr.offset) (SZ.v arr.offset + Seq.length s0) #(p0) s0);
@@ -207,6 +312,89 @@ fn gather
     A.pts_to_range_gather a #_ #_ #s0 #s1 #p0 #p1;
     rewrite (A.pts_to_range a (SZ.v arr.offset) (SZ.v arr.offset + Seq.length s0) #(p0 +. p1) s0)
       as pts_to arr #(p0 +. p1) s0
+  } else {
+    let test = (offset arr = 0 && Seq.length (Ghost.reveal s0) = 1);
+    if (test) {
+      let Ref a = arr.base;
+      rewrite (pts_to arr #p0 s0)
+        as (R.pts_to a #p0 (Seq.index s0 0));
+      rewrite (pts_to arr #p1 s1)
+        as (R.pts_to a #p1 (Seq.index s1 0));
+      R.gather a;
+      assert (pure (Seq.equal s0 s1));
+      rewrite (R.pts_to a #(p0 +. p1) (Seq.index s0 0))
+        as (pts_to arr #(p0 +. p1) s0);
+    } else {
+      rewrite (pts_to arr #p0 s0)
+        as (v_is_empty arr s0);
+      unfold (v_is_empty arr s0);
+      rewrite (pts_to arr #p1 s1)
+        as (v_is_empty arr s1);
+      unfold (v_is_empty arr s1);
+      assert (pure (Seq.equal s0 s1));
+      fold (v_is_empty arr s0);
+      rewrite (v_is_empty arr s0)
+        as (pts_to arr #(p0 +. p1) s0);
+    }
+  }
+}
+
+let shift
+  (#t: Type) (s: ptr t) (i: SZ.t { SZ.v s.offset + SZ.v i <= base_length s.base })
+: Tot (ptr t)
+= 
+  {
+        base = s.base;
+        offset = SZ.add s.offset i;
+  }
+
+ghost fn ghost_shift (#t: Type) (s: ptr t) (#p: perm) (i: SZ.t)
+    (#v: Ghost.erased (Seq.seq t) { SZ.v i <= Seq.length v })
+  requires pts_to s #p v
+  returns res: squash (SZ.v s.offset + SZ.v i <= base_length s.base)
+  ensures
+    pts_to s #p (Seq.slice v 0 (SZ.v i)) **
+    pts_to (shift s i) #p (Seq.slice v (SZ.v i) (Seq.length v))
+{
+    pts_to_not_null s;
+  if (Array? s.base) {
+    let Array a = s.base;
+    rewrite pts_to s #p v
+      as A.pts_to_range a (SZ.v s.offset) (SZ.v s.offset + Seq.length v) #p v;
+    A.pts_to_range_prop a;
+    let s' = shift s i;
+    A.pts_to_range_split a _ (SZ.v s'.offset) _;
+    with s1. assert A.pts_to_range a (SZ.v s.offset) (SZ.v s'.offset) #p s1;
+    rewrite
+        (A.pts_to_range a (SZ.v s.offset) (SZ.v s'.offset) #p s1)
+        as pts_to s #p s1;
+    with s2. assert A.pts_to_range a (SZ.v s'.offset) (SZ.v s.offset + Seq.length v) #p s2;
+    rewrite
+        (A.pts_to_range a (SZ.v s'.offset) (SZ.v s.offset + Seq.length v) #p s2)
+        as pts_to (shift s i) #p s2;
+    ()
+  } else {
+    pts_to_length s;
+    let res : squash (SZ.v s.offset + SZ.v i <= base_length s.base) = ();
+    let Ref a = s.base;
+    let test = (SZ.v i + 1 <= Seq.length v);
+    if (test) {
+      assert (pure (Seq.equal v (Seq.slice v (SZ.v i) (Seq.length v))));
+      rewrite pts_to s #p v
+        as pts_to (shift s i) #p (Seq.slice v (SZ.v i) (Seq.length v));
+      fold (v_is_empty s (Seq.slice v 0 (SZ.v i)));
+      rewrite (v_is_empty s (Seq.slice v 0 (SZ.v i)))
+        as pts_to s #p (Seq.slice v 0 (SZ.v i));
+    } else {
+      assert (pure (Seq.equal v (Seq.slice v 0 (SZ.v i))));
+      rewrite pts_to s #p v
+        as pts_to s #p (Seq.slice v 0 (SZ.v i));
+      fold (v_is_empty s (Seq.slice v (SZ.v i) (Seq.length v)));
+      rewrite (v_is_empty s (Seq.slice v (SZ.v i) (Seq.length v)))
+        as pts_to (shift s i) #p (Seq.slice v (SZ.v i) (Seq.length v));
+      res
+    }
+  }
 }
 
 fn split (#t: Type) (s: ptr t) (#p: perm) (i: SZ.t)
@@ -218,25 +406,8 @@ fn split (#t: Type) (s: ptr t) (#p: perm) (i: SZ.t)
     pts_to s' #p (Seq.slice v (SZ.v i) (Seq.length v)) **
     pure (adjacent s (SZ.v i) s')
 {
-    pts_to_not_null s;
-    let Array a = s.base;
-    rewrite pts_to s #p v
-      as A.pts_to_range a (SZ.v s.offset) (SZ.v s.offset + Seq.length v) #p v;
-    A.pts_to_range_prop a;
-    let s' = {
-        base = s.base;
-        offset = SZ.add s.offset i;
-    };
-    A.pts_to_range_split a _ (SZ.v s'.offset) _;
-    with s1. assert A.pts_to_range a (SZ.v s.offset) (SZ.v s'.offset) #p s1;
-    rewrite
-        (A.pts_to_range a (SZ.v s.offset) (SZ.v s'.offset) #p s1)
-        as pts_to s #p s1;
-    with s2. assert A.pts_to_range a (SZ.v s'.offset) (SZ.v s.offset + Seq.length v) #p s2;
-    rewrite
-        (A.pts_to_range a (SZ.v s'.offset) (SZ.v s.offset + Seq.length v) #p s2)
-        as pts_to s' #p s2;
-    s'
+    ghost_shift s i;
+    shift s i
 }
 
 ghost fn ghost_split (#t: Type) (s: ptr t) (#p: perm) (i: SZ.t)
@@ -248,25 +419,8 @@ ghost fn ghost_split (#t: Type) (s: ptr t) (#p: perm) (i: SZ.t)
     pts_to (reveal s') #p (Seq.slice v (SZ.v i) (Seq.length v)) **
     pure (adjacent s (SZ.v i) s')
 {
-    pts_to_not_null s;
-    let Array a = s.base;
-    rewrite pts_to s #p v
-      as A.pts_to_range a (SZ.v s.offset) (SZ.v s.offset + Seq.length v) #p v;
-    A.pts_to_range_prop a;
-    let s' = {
-        base = s.base;
-        offset = SZ.add s.offset i;
-    };
-    A.pts_to_range_split a _ (SZ.v s'.offset) _;
-    with s1. assert A.pts_to_range a (SZ.v s.offset) (SZ.v s'.offset) #p s1;
-    rewrite
-        (A.pts_to_range a (SZ.v s.offset) (SZ.v s'.offset) #p s1)
-        as pts_to s #p s1;
-    with s2. assert A.pts_to_range a (SZ.v s'.offset) (SZ.v s.offset + Seq.length v) #p s2;
-    rewrite
-        (A.pts_to_range a (SZ.v s'.offset) (SZ.v s.offset + Seq.length v) #p s2)
-        as pts_to s' #p s2;
-    s'
+    ghost_shift s i;
+    shift s i
 }
 
 
@@ -276,6 +430,7 @@ fn join (#t: Type) (s1: ptr t) (#p: perm) (#v1: Seq.seq t) (s2: ptr t) (#v2: Seq
     ensures pts_to s1 #p (Seq.append v1 v2)
 {
     pts_to_not_null s1;
+  if (Array? s1.base) {
     let Array a = s1.base;
     rewrite pts_to s1 #p v1
       as (A.pts_to_range a (SZ.v s1.offset) (SZ.v s1.offset + Seq.length v1) #p v1);
@@ -284,9 +439,23 @@ fn join (#t: Type) (s1: ptr t) (#p: perm) (#v1: Seq.seq t) (s2: ptr t) (#v2: Seq
     A.pts_to_range_join a (SZ.v s1.offset) (SZ.v s1.offset + Seq.length v1) (SZ.v s1.offset + Seq.length v1 + Seq.length v2);
     rewrite (A.pts_to_range a (SZ.v s1.offset) (SZ.v s1.offset + Seq.length v1 + Seq.length v2) #p (Seq.append v1 v2))
     as pts_to s1 #p (Seq.append v1 v2)
+  } else {
+    pts_to_length s1;
+    pts_to_length s2;
+    if (Seq.length v2 = 0) {
+      rewrite pts_to s2 #p v2 as v_is_empty s2 v2;
+      unfold v_is_empty s2 v2;
+      assert (pure (Seq.equal v1 (Seq.append v1 v2)));
+      rewrite pts_to s1 #p v1 as pts_to s1 #p (Seq.append v1 v2);
+    } else {
+      let Ref a = s1.base;
+      rewrite pts_to s1 #p v1 as v_is_empty s1 v1;
+      unfold v_is_empty s1 v1;
+      assert (pure (Seq.equal v2 (Seq.append v1 v2)));
+      rewrite pts_to s2 #p v2 as pts_to s1 #p (Seq.append v1 v2);
+    }
+  }
 }
-
-module R = Pulse.Lib.Reference
 
 fn memcpy
     (#t:Type0) (#p0:perm)
