pulse/src/extraction/ExtractPulse.fst
@@ -165,7 +165,9 @@ let pulse_translate_expr : translate_expr_t = fun env e ->
     EBufRead (translate_expr env e, translate_expr env i)
 
   | MLE_App ({ expr = MLE_TApp({ expr = MLE_Name p }, _) }, [ x; _p; _w ])
-    when string_of_mlpath p = "Pulse.Lib.ArrayPtr.from_array" ->
+    when
+      string_of_mlpath p = "Pulse.Lib.ArrayPtr.from_ref" ||
+      string_of_mlpath p = "Pulse.Lib.ArrayPtr.from_array" ->
     translate_expr env x
 
   | MLE_App ({ expr = MLE_TApp({ expr = MLE_Name p }, _) }, [ a; _p; i; _w ])
